Working STLC!

rupicola/io/STLC.fst
@@ -270,62 +270,73 @@ type step : closed_exp -> closed_exp -> (h:history) -> option (event_h h) -> Typ
     e2:value ->
     h:history ->
     step (EApp (ELam e11) e2) (subst_beta e2 e11) h None
-  (*| IfCond :
+  | IfCond :
     #e1:closed_exp ->
     e2:closed_exp ->
     e3:closed_exp ->
     #e1':closed_exp ->
-    #oev:option event ->
-    hst:step e1 e1' oev ->
-    step (EIf e1 e2 e3) (EIf e1' e2 e3) oev
+    #h:history ->
+    #oev:option (event_h h) ->
+    hst:step e1 e1' h oev ->
+    step (EIf e1 e2 e3) (EIf e1' e2 e3) h oev
   | IfTrue :
     e2:closed_exp ->
     e3:closed_exp ->
-    step (EIf ETrue e2 e3) e2 None
+    h:history ->
+    step (EIf ETrue e2 e3) e2 h None
   | IfFalse :
     e2:closed_exp ->
     e3:closed_exp ->
-    step (EIf EFalse e2 e3) e3 None
+    h:history ->
+    step (EIf EFalse e2 e3) e3 h None
   | PairLeft :
     #e1:closed_exp ->
     e2:closed_exp ->
     #e1':closed_exp ->
-    #oev:option event ->
-    hst:step e1 e1' oev ->
-    step (EPair e1 e2) (EPair e1' e2) oev
+    #h:history ->
+    #oev:option (event_h h) ->
+    hst:step e1 e1' h oev ->
+    step (EPair e1 e2) (EPair e1' e2) h oev
   | PairRight :
     e1:closed_exp{is_value e1} ->
     #e2:closed_exp ->
     #e2':closed_exp ->
-    #oev:option event ->
-    hst:step e2 e2' oev ->
-    step (EPair e1 e2) (EPair e1 e2') oev
+    #h:history ->
+    #oev:option (event_h h) ->
+    hst:step e2 e2' h oev ->
+    step (EPair e1 e2) (EPair e1 e2') h oev
   | FstPair :
     #e':closed_exp ->
     #e'':closed_exp ->
-    #oev:option event ->
-    hst:step e' e'' oev ->
-    step (EFst e') (EFst e'') oev
+    #h:history ->
+    #oev:option (event_h h) ->
+    hst:step e' e'' h oev ->
+    step (EFst e') (EFst e'') h oev
   | FstPairReturn :
     #e1:closed_exp{is_value e1} ->
     #e2:closed_exp{is_value e2} ->
-    step (EFst (EPair e1 e2)) e1 None
+    h:history ->
+    step (EFst (EPair e1 e2)) e1 h None
   | SndPair :
     #e':closed_exp ->
     #e'':closed_exp ->
-    #oev:option event ->
-    hst:step e' e'' oev ->
-    step (ESnd e') (ESnd e'') oev
+    #h:history ->
+    #oev:option (event_h h) ->
+    hst:step e' e'' h oev ->
+    step (ESnd e') (ESnd e'') h oev
   | SndPairReturn :
     #e1:closed_exp{is_value e1} ->
     #e2:closed_exp{is_value e2} ->
-    step (ESnd (EPair e1 e2)) e2 None
+    h:history ->
+    step (ESnd (EPair e1 e2)) e2 h None
   | SRead :
     b:bool ->
-    step ERead (get_ebool b) (Some (EvRead () (Some b)))
+    h:history ->
+    step ERead (get_ebool b) h (Some (EvRead () (Some b)))
   | SWrite :
     b:bool ->
-    step (EWrite (get_ebool b)) EUnit (Some (EvWrite b (Some ())))*)
+    h:history ->
+    step (EWrite (get_ebool b)) EUnit h (Some (EvWrite b (Some ())))
 
 let can_step (e:closed_exp) (h:history) : Type0 =
   exists (e':closed_exp) (oev:option (event_h h)). step e e' h oev
@@ -334,48 +345,32 @@ let irred (e:closed_exp) (h:history) : Type0 =
   forall (e':closed_exp) (oev:option (event_h h)). ~(step e e' h oev) 
   // optionally \/ is_value e - Amal's definition
 
-(*let rec lem_value_is_irred (e:closed_exp) : Lemma
+let rec lem_value_is_irred (e:closed_exp) (h:history) : Lemma
   (requires is_value e)
-  (ensures irred e)
-  [SMTPat (irred e)] =
+  (ensures (irred e h))
+  [SMTPat (irred e h)] = 
   match e with
   | EUnit ->
-    assert (forall e' oev. ~(step EUnit e' oev)) by explode ()
+    assert (forall e' oev. ~(step EUnit e' h oev)) by explode ()
   | ETrue ->
-    assert (forall e' oev. ~(step ETrue e' oev)) by explode ()
+    assert (forall e' oev. ~(step ETrue e' h oev)) by explode ()
   | EFalse ->
-    assert (forall e' oev. ~(step EFalse e' oev)) by explode ()
+    assert (forall e' oev. ~(step EFalse e' h oev)) by explode ()
   | ELam e11 ->
-    assert (forall e' oev. ~(step (ELam e11) e' oev)) by explode ()
+    assert (forall e' oev. ~(step (ELam e11) e' h  oev)) by explode ()
   | EPair e1 e2 ->
-    lem_value_is_irred e1;
-    lem_value_is_irred e2;
-    introduce forall (e':closed_exp) (oev:option event). step e e' oev ==> False with begin
-      introduce step e e' oev ==> False with h. begin
-        FStar.Squash.bind_squash #(step e e' oev) () (fun st ->
+    lem_value_is_irred e1 h;
+    lem_value_is_irred e2 h;
+    introduce forall (e':closed_exp) (oev:option (event_h h)). step e e' h oev ==> False with begin
+      introduce step e e' h oev ==> False with _. begin
+        FStar.Squash.bind_squash #(step e e' h oev) () (fun st ->
         match st with
         | PairLeft e2 hst -> ()
         | PairRight e1 hst -> ()
         | _ -> ())
       end
     end
-  | _ -> ()*)
-
-(*let rec compute_lt (lt:local_trace []) (oev:option event) : local_trace [] = 
-   if Some? oev then begin
-   let lt' = ((Some?.v oev)::lt) in
-   assume (test_event [] (Some?.v oev));
-   lt'
-   end
-   else lt*)
-
-(*let rec compute_lt' (h:history) (lt:local_trace h) : Tot (local_trace []) (decreases lt) =
-  match lt with
-  | [] -> []
-  | ev' :: tl -> ev' :: (compute_lt' (ev'::h) tl)*)
-
-//let compute_lt (oev:option event) (h:history) : local_trace h =
-//    if Some? oev then [Some?.v oev] else []
+  | _ -> ()
 
 (** reflexive transitive closure of step *)
 noeq
@@ -392,12 +387,6 @@ type steps : closed_exp -> closed_exp -> (h:history) -> local_trace h -> Type =
            step e1 e2 h oev ->
            steps e2 e3 (if Some? oev then (Some?.v oev)::h else h) lt ->
            steps e1 e3 h (if Some? oev then [Some?.v oev] @ lt else lt)
-
-(*let trans_well_formed_local_trace_steps (e e':closed_exp) (h:trace) (lt:local_trace h) (lt1:local_trace (h++lt)) :
-  Lemma (requires steps e e' (h++lt) lt1)
-        (ensures steps e e' h (
-        *)
-  
 
 // how would we check the compatability of two histories? saying that there exists an ordering of the events that is well-formed?
 let rec lem_steps_transitive_constructive
@@ -600,6 +589,9 @@ let can_step_eapp_when_safe (e1 e2:closed_exp) (t1 t2:typ) (h:history) : Lemma
        Subsubcase irred e2. (From safe e2 we get is_value e2; but not needed by step.)
          So e = EApp (ELam e11) e2 -> subst_beta e2 e11 = e''. Return e11 e2. *)
 
+let get_event_trace (#h:history) (oev:option (event_h h)) : local_trace h = 
+  if Some? oev then [Some?.v oev] else []
+
 let rec destruct_steps_eapp
   (e1:closed_exp)
   (e2:closed_exp)
@@ -610,7 +602,7 @@ let rec destruct_steps_eapp
   (t1:typ)
   (t2:typ) :
   Pure (exp * value * (lt2:local_trace h & (lt1:local_trace (h++lt2) & local_trace (((h++lt2)++lt1)))))
-    (requires irred e' h /\ (** CH: needed, otherwise I can take zero steps; could be replaced by value e' *)
+    (requires irred e' (h++lt) /\ (** CH: needed, otherwise I can take zero steps; could be replaced by value e' *)
       safe e1 /\
       sem_expr_shape (TArr t1 t2) e1 /\
       safe e2)
@@ -621,8 +613,8 @@ let rec destruct_steps_eapp
       steps (EApp e1 e2) (subst_beta e2' e11) h (lt2 @ lt1) /\
       steps (subst_beta e2' e11) e' ((h++lt2)++lt1) lt3 /\
       lt == ((lt2 @ lt1) @ lt3) /\
-      (irred e2 h ==> lt2 == []) /\
-      (irred e1 (h++lt2) ==> lt1 == []))
+      (irred e2 h ==> (lt2 == [] /\ e2 == e2')) /\
+      (irred e1 (h++lt2) ==> (lt1 == [] /\ e1 == ELam e11)))
     (decreases st)
   =  match st with
     | SRefl (EApp e1 e2) h -> begin
@@ -634,257 +626,148 @@ let rec destruct_steps_eapp
     | STrans #e #f2 #e' #h #_ #lt23 step_eapp step_eapp_steps -> begin
       let (EApp e1 e2) = e in
       match step_eapp with
+      | AppLeft #e1 e2 #e1' #h #oev1 step_e1 -> begin
+        let (EApp e1' e2) = f2 in
+        lem_step_implies_steps e1 e1' h oev1;
+        lem_step_implies_steps (EApp e1 e2) (EApp e1' e2) h oev1;
+        let lt1 : local_trace h = get_event_trace oev1 in
+        lem_steps_preserve_safe e1 e1' h lt1;
+        lem_steps_preserve_sem_expr_shape e1 e1' h lt1 (TArr t1 t2);
+        let s2 : steps (EApp e1' e2) e' (h++lt1) lt23 = step_eapp_steps in
+        let (e11, e2', (| _, (| lt1', lt3 |) |)) = destruct_steps_eapp e1' e2 e' (h++lt1) lt23 s2 t1 t2 in
+        lem_steps_transitive e1 e1' (ELam e11) h lt1 lt1';
+        lem_steps_transitive (EApp e1 e2) (EApp e1' e2) (subst_beta e2' e11) h lt1 lt1';
+        (e11, e2', (| [] , (| (lt1 @ lt1'), lt3 |) |))
+        end
       | AppRight e1 #e2 #e2' #h #oev2 step_e2 -> begin
         let (EApp e1 e2') = f2 in
         lem_step_implies_steps e2 e2' h oev2;
         lem_step_implies_steps (EApp e1 e2) (EApp e1 e2') h oev2;
-        match oev2 with
-        | Some ev -> 
-          let lt2 : local_trace h = [ev] in
-          lem_steps_preserve_safe e2 e2' h lt2;
-          let s2 : steps (EApp e1 e2') e' (h++[ev]) lt23 = step_eapp_steps in
-          assume (irred e' (h++[ev]));
-          assert (lt == ([ev] @ lt23));
-          let (e11, e2'', (| lt2', (| lt1, lt3 |) |)) = destruct_steps_eapp e1 e2' e' (h++[ev]) lt23 s2 t1 t2 in
-          //lem_steps_transitive e2 e2' e2'' h lt2 lt2';
-          let lt2'' : local_trace h = ([ev] @ lt2') in
-          //trans_well_formed_local_trace 
-          //let lt1' : local_trace (h++lt2') = lt1 in
-          //lem_steps_transitive (EApp e1 e2) (EApp e1 e2') h lt2 lt2';
-          (e11, e2'', (| lt2'', (| lt1, lt3 |) |))
-          //admit ()
-        | None -> admit ()
+        let lt2 : local_trace h = get_event_trace oev2 in
+        lem_steps_preserve_safe e2 e2' h lt2;
+        let s2 : steps (EApp e1 e2') e' (h++lt2) lt23 = step_eapp_steps in
+        let (e11, e2'', (| lt2', (| lt1, lt3 |) |)) = destruct_steps_eapp e1 e2' e' (h++lt2) lt23 s2 t1 t2 in
+        lem_steps_transitive e2 e2' e2'' h lt2 lt2';
+        lem_steps_transitive (EApp e1 e2) (EApp e1 e2') (subst_beta e2'' e11) h lt2 (lt2' @ lt1);
+        (e11, e2'', (| (lt2 @ lt2'), (| lt1, lt3 |) |))
         end
-      | _ -> admit ()
-      end
-       (*| AppLeft #e1 e2 #e1' #h #oev1 step_e1 -> begin
-        let (EApp e1' e2) = f2 in
-        lem_step_implies_steps e1 e1' h oev1;
-        lem_step_implies_steps (EApp e1 e2) (EApp e1' e2) h oev1;
-        //let lt1 : local_trace h = (if Some? oev then [Some?.v oev] else []) in        
-        match oev1 with 
-        | Some ev -> 
-          let lt1 : local_trace h = [ev] in
-          lem_steps_preserve_safe e1 e1' h lt1;
-          lem_steps_preserve_sem_expr_shape e1 e1' h lt1 (TArr t1 t2);
-          let s2 : steps (EApp e1' e2) e' (h++[ev]) lt23 = step_eapp_steps in
-          assume (irred e' (h++[ev]));
-          let (e11, e2', (| _, (| lt1', lt3 |) |)) = destruct_steps_eapp e1' e2 e' (h++[ev]) lt23 s2 t1 t2 in
-          assume (irred e2 (h++[ev]));
-          let lt3 : local_trace ((h++[ev])++lt1') = lt3 in
-          let lt1' : local_trace (h++[ev]) = lt1' in
-          let lt1 : local_trace h = [ev] in
-          lem_steps_transitive e1 e1' (ELam e11) h lt1 lt1';
-          let lt3 : local_trace ((h++[ev])++lt1') = lt3 in
-          let lt3_a : local_trace (h++[ev]) = (lt1' @ lt3) in 
-          let lt3_b : local_trace h = ([ev] @ (lt1' @ lt3)) in
-          let lt3_c : local_trace h = (([ev] @ lt1') @ lt3) in
-          test_lemma h ev lt1' lt3;
-          let lt3_d : local_trace (h++([ev] @ lt1')) = lt3 in
-          assume (steps e2 e2' h []);
-          assert (is_closed (ELam e11));
-          assert (steps e1 (ELam e11) h ([ev] @ lt1'));
-          assume (steps (EApp e1 e2) (subst_beta e2' e11) h ([ev] @ lt1'));
-          assume (steps (subst_beta e2' e11) e' (h++([ev] @ lt1')) lt3_d);
-          assert (lt == (([ev] @ lt1') @ lt3_d));
-          assert (irred e2 h ==> True);
-          assert (irred e1 h ==> ([ev] ++ lt1') == []);
-          (e11, e2', (| [] , (| ([ev] @ lt1'), lt3_d |) |)) 
-          // lt1' : local_trace (h++[ev])
-          // lt1'': local_trace h
-          // lt3: local_trace ((h++[ev])++lt1')
-          // lt3'': local_trace (h++lt1'')                                                  
-       | None ->
-          let lt1 : local_trace h = [] in
-          lem_steps_preserve_safe e1 e1' h lt1;
-          lem_steps_preserve_sem_expr_shape e1 e1' h lt1 (TArr t1 t2);
-          let s2 : steps (EApp e1' e2) e' h lt23 = step_eapp_steps in
-          let (e11, e2', (| _, (| lt1', lt3 |) |)) = destruct_steps_eapp e1' e2 e' h lt23 s2 t1 t2 in
-          //assert (steps e2 e2 h []);
-          assume (irred e2 h);
-          lem_steps_transitive e1 e1' (ELam e11) h lt1 lt1';
-          lem_steps_transitive (EApp e1 e2) (EApp e1' e2) (subst_beta e2' e11) h lt1 lt1';
-          (e11, e2', (| [] , (| lt1', lt3 |) |))
-        end*)  
-     
-
-
-
-
-
-
-
-
-
-        (*let lt1 : local_trace h = (if Some? oev1 then [Some?.v oev1] else []) in
-        lem_steps_preserve_safe e1 e1' h lt1;
-        lem_steps_preserve_sem_expr_shape e1 e1' h lt1 (TArr t1 t2);
-        let h' = if Some? oev1 then h++[Some?.v oev1] else h in
-        let s2 : steps (EApp e1' e2) e' h' lt_f2_f3 = step_eapp_steps in
-        assume (irred e' h');
-        assert (safe e1');
-        assert (sem_expr_shape (TArr t1 t2) e1');
-        assert (safe e2);
-        let (e11'', e2'', (| lt2'', (| lt1'', lt3'' |) |)) = destruct_steps_eapp e1' e2 e' h' lt_f2_f3 s2 t1 t2 in
-        //trans_well_formed_local_trace h' lt2'' lt1'';
-        //assert (well_formed_local_trace h' (lt2'' @ lt1''));
-        let _ : local_trace (h'++lt2'') = lt1'' in
-        lem_steps_transitive e1 e1' (ELam e11'') h lt1 lt1'';
-        admit ()
+      | Beta e11 e2 h -> begin
+        lem_step_implies_steps (EApp e1 e2) (subst_beta e2 e11) h None;
+        (e11, e2, (| [], (| [], lt |) |))
         end
-      | _ -> admit ()
       end
 
-        
-        end
-      | _ -> admit ()
-      end*)
-      
-      (*| AppRight e1 #e2 #e2' step_e2 -> begin
-        let (EApp e1 e2') = f2 in
-        lem_step_implies_steps e2 e2';
-        lem_step_implies_steps (EApp e1 e2) (EApp e1 e2');
-        lem_steps_preserve_safe e2 e2';
-        let s2 : steps (EApp e1 e2') e' = step_eapp_steps in
-        let (e11'', e2'') = destruct_steps_eapp e1 e2' e' s2 t1 t2 in
-        lem_steps_transitive e2 e2' e2'';
-        lem_steps_transitive (EApp e1 e2) (EApp e1 e2') (subst_beta e2'' e11'');
-        (e11'', e2'')
-        end
-      | Beta e11 e2 -> begin
-        lem_step_implies_steps (EApp e1 e2) (subst_beta e2 e11);
-        (e11, e2)
-        end
-      | _ -> false_elim ()
-      end
-    *)
-
-let can_step_eif_when_safe (e1 e2 e3:closed_exp) : Lemma
+let can_step_eif_when_safe (e1 e2 e3:closed_exp) (h:history) : Lemma
   (requires
     safe e1 /\
     sem_expr_shape TBool e1)
-  (ensures (exists e' oev. step (EIf e1 e2 e3) e' oev))
-  = admit ()
-  (*introduce irred e1 /\ e1 == ETrue ==> (exists e' oev. step (EIf e1 e2 e3) e' oev) with _.
-  begin
-    assert (steps e1 e1 []);
-    let st : step (EIf ETrue e2 e3) e2 None = IfTrue e2 e3 in
+  (ensures (exists e' oev. step (EIf e1 e2 e3) e' h oev))
+  = 
+  introduce irred e1 h /\ e1 == ETrue ==> (exists e' oev. step (EIf e1 e2 e3) e' h oev) with _. begin
+    assert (steps e1 e1 h []);
+    let st : step (EIf ETrue e2 e3) e2 h None = IfTrue e2 e3 h in
     ()
   end;
   
-  introduce irred e1 /\ e1 == EFalse ==> (exists e' oev. step (EIf e1 e2 e3) e' oev) with _.
-  begin
-    assert (steps e1 e1 []);
-    let st : step (EIf EFalse e2 e3) e3 None = IfFalse e2 e3 in
+  introduce irred e1 h /\ e1 == EFalse ==> (exists e' oev. step (EIf e1 e2 e3) e' h oev) with _. begin
+    assert (steps e1 e1 h []);
+    let st : step (EIf EFalse e2 e3) e3 h None = IfFalse e2 e3 h in
     ()
   end;
   
-  introduce ~(irred e1) ==> (exists e' oev. step (EIf e1 e2 e3) e' oev) with _.
-  begin
-    assert (exists e1' oev1. step e1 e1' oev1);
-    eliminate exists e1' oev1. step e1 e1' oev1 returns exists e' oev. step (EIf e1 e2 e3) e' oev with st. begin
-      bind_squash st (fun st -> return_squash (IfCond e2 e3 st));
-      assume (exists e' oev. step (EIf e1 e2 e3) e' oev)
-      //bind_squash st (fun st -> return_squash (IfCond e2 e3 st));
+  introduce irred e1 h /\ ~(e1 == EFalse \/ e1 == ETrue) ==> (exists e' oev. step (EIf e1 e2 e3) e' h oev) with _. begin
+    assert (steps e1 e1 h []);
+    false_elim ()
+  end;
+  
+  introduce ~(irred e1 h) ==> (exists e' oev. step (EIf e1 e2 e3) e' h oev) with _. begin
+    assert (exists e1' oev1. step e1 e1' h oev1);
+    eliminate exists e1' oev1. step e1 e1' h oev1 returns exists e' oev. step (EIf e1 e2 e3) e' h oev with st. begin
+      bind_squash st (fun st -> return_squash (IfCond e2 e3 st))
     end
-  end*)
+  end
 
 let rec destruct_steps_eif
   (e1:closed_exp)
   (e2:closed_exp)
   (e3:closed_exp)
   (e':closed_exp)
-  (lt:local_trace [])
-  (st:steps (EIf e1 e2 e3) e' lt) :
-  Pure (closed_exp * local_trace [] * local_trace [] * local_trace [])
-    (requires irred e' /\
+  (h:history)
+  (lt:local_trace h)
+  (st:steps (EIf e1 e2 e3) e' h lt) :
+  Pure (closed_exp * (lt1:local_trace h & (local_trace (h++lt1) * local_trace (h++lt1))))
+    (requires irred e' (h++lt) /\
       safe e1 /\
       sem_expr_shape TBool e1) (** CA: not sure if necessary **)
-    (ensures fun (e1', lt1, lt2, lt3) ->
-      irred e1' /\
-      steps e1 e1' lt1 /\
-      steps (EIf e1 e2 e3) (EIf e1' e2 e3) lt1 /\
-      (ETrue? e1' ==> steps e2 e' lt2) /\
-      (EFalse? e1' ==> steps e3 e' lt3) /\
-      ((lt == lt1 @ lt2) \/ (lt == lt1 @ lt3)))
+    (ensures fun (e1', (| lt1, (lt2, lt3) |)) ->
+      irred e1' (h++lt1) /\
+      steps e1 e1' h lt1 /\
+      steps (EIf e1 e2 e3) (EIf e1' e2 e3) h lt1 /\
+      (ETrue? e1' ==> steps e2 e' (h++lt1) lt2) /\
+      (EFalse? e1' ==> steps e3 e' (h++lt1) lt3) /\
+      ((lt == lt1 @ lt2) \/ (lt == lt1 @ lt3)) /\
+      (irred e1 h ==> (lt1 == [] /\ e1 == e1')))
     (decreases st)
-  = admit ()
-    (*match st with
-    | SRefl (EIf e1 e2 e3) -> begin
-      can_step_eif_when_safe e1 e2 e3;
+  = match st with
+    | SRefl (EIf e1 e2 e3) h -> begin
+      can_step_eif_when_safe e1 e2 e3 h;
       false_elim ()
       end
-    | STrans #f1 #f2 #f3 #lt_f2_f3 #oev_f1_f2 step_eif step_eif_steps -> begin
-      let (EIf e1 e2 e3) = f1 in
-      let e' = f3 in
+    | STrans #e #f2 #e' #h #_ #lt23 step_eif step_eif_steps -> begin
+      let (EIf e1 e2 e3) = e in
       match step_eif with
-      | IfCond #e1 e2 e3 #e1' #oev1 step_e1 -> begin
+      | IfCond #e1 e2 e3 #e1' #h #oev1 step_e1 -> begin
         let (EIf e1' e2 e3) = f2 in
-        assume (Some? oev1 ==> well_formed_local_trace [] [Some?.v oev1]);
-        lem_step_implies_steps e1 e1' oev1;
-        lem_step_implies_steps (EIf e1 e2 e3) (EIf e1' e2 e3) oev1;
-        let lt1 = (if Some? oev1 then ([] @ [Some?.v oev1]) else []) in
-        lem_steps_preserve_safe e1 e1' lt1;
-        lem_steps_preserve_sem_expr_shape e1 e1' lt1 TBool;
-        let s2 : steps (EIf e1' e2 e3) e' lt_f2_f3 = step_eif_steps in
-        let (e1'', lt1'', lt2'', lt3'') = destruct_steps_eif e1' e2 e3 e' lt_f2_f3 s2 in
-        assume (well_formed_local_trace (List.rev lt1) lt1'');
-        lem_steps_transitive e1 e1' e1'' lt1 lt1'';
-        lem_steps_transitive (EIf e1 e2 e3) (EIf e1' e2 e3) (EIf e1'' e2 e3) lt1 lt1'';
-        assert (irred e1'');
-        assert (steps e1 e1'' lt1'');
-        assume (steps (EIf e1 e2 e3) (EIf e1'' e2 e3) lt1'');
-        assume (ETrue? e1'' ==> steps e2 e' lt2'');
-        assume (EFalse? e1'' ==> steps e3 e' lt3'');
-        assume ((lt == lt1'' @ lt2'') \/ (lt == lt1'' @ lt3''));
-        (e1'', lt1'', lt2'', lt3'')
+        lem_step_implies_steps e1 e1' h oev1;
+        lem_step_implies_steps (EIf e1 e2 e3) (EIf e1' e2 e3) h oev1;
+        let lt1 : local_trace h = get_event_trace oev1 in
+        lem_steps_preserve_safe e1 e1' h lt1;
+        lem_steps_preserve_sem_expr_shape e1 e1' h lt1 TBool;
+        let s2 : steps (EIf e1' e2 e3) e' (h++lt1) lt23 = step_eif_steps in
+        let (e1'', (| lt1', (lt2, lt3) |)) = destruct_steps_eif e1' e2 e3 e' (h++lt1) lt23 s2 in
+        lem_steps_transitive e1 e1' e1'' h lt1 lt1';
+        lem_steps_transitive (EIf e1 e2 e3) (EIf e1' e2 e3) (EIf e1'' e2 e3) h lt1 lt1';
+        (e1'', (| (lt1 @ lt1'), (lt2, lt3) |))
         end
-      | _ -> admit ()
+      | IfTrue e2 e3 h -> begin
+        lem_step_implies_steps (EIf e1 e2 e3) e2 h None;
+        assert (steps e1 e1 h []);
+        (e1, (| [], (lt, []) |))
+        end
+      | IfFalse e2 e3 h -> begin
+        lem_step_implies_steps (EIf e1 e2 e3) e3 h None;
+        assert (steps e1 e1 h []);
+        (e1, (| [], ([], lt) |))
+        end
       end
-      
-      | IfTrue e2 e3 -> begin
-        lem_step_implies_steps (EIf e1 e2 e3) e2;
-        e1
-        end
-      | IfFalse e2 e3 -> begin
-        lem_step_implies_steps (EIf e1 e2 e3) e3;
-        e1
-        end
-      | _ -> false_elim ()
-      end*)
 
   (**
     How the steps look like:
       EIf e1 e2 e3 -->* EIf e1' e2 e3 -->* e'
   **)
 
-let srefl_epair_implies_value (e1 e2:closed_exp) : Lemma
-  (requires safe e1 /\ safe e2 /\ irred (EPair e1 e2))
+let srefl_epair_implies_value (e1 e2:closed_exp) (h:history) : Lemma
+  (requires safe e1 /\ safe e2 /\ irred (EPair e1 e2) h)
   (ensures is_value (EPair e1 e2))
   =
-  introduce irred e1 /\ irred e2 ==> is_value (EPair e1 e2) with _.
-  begin 
-    assert (steps e1 e1 []);
-    assert (steps e2 e2 []);
+  introduce irred e1 h /\ irred e2 h ==> is_value (EPair e1 e2) with _. begin 
+    assert (steps e1 e1 h []);
+    assert (steps e2 e2 h []);
     ()
   end;
   
-  introduce ~(irred e1) ==> is_value (EPair e1 e2) with _.
-  begin
-    assert (exists e1' oev1. step e1 e1' oev1);
-    eliminate exists e1' oev1. step e1 e1' oev1 returns exists e' oev. step (EPair e1 e2) e' oev with st.
-    begin
+  introduce ~(irred e1 h) ==> is_value (EPair e1 e2) with _. begin
+    assert (exists e1' oev1. step e1 e1' h oev1);
+    eliminate exists e1' oev1. step e1 e1' h oev1 returns exists e' oev. step (EPair e1 e2) e' h oev with st. begin
       bind_squash st (fun st -> return_squash (PairLeft e2 st))
     end;
     false_elim ()
   end;
-  
-  introduce irred e1 /\ ~(irred e2) ==> is_value (EPair e1 e2) with _.
-  begin
-    assert (steps e1 e1 []);
-    assert (exists e2' oev2. step e2 e2' oev2);
-    eliminate exists e2' oev2. step e2 e2' oev2 returns exists e' oev. step (EPair e1 e2) e' oev with st.
-    begin
+
+  introduce irred e1 h /\ ~(irred e2 h) ==> is_value (EPair e1 e2) with _. begin
+    assert (steps e1 e1 h []);
+    assert (exists e2' oev2. step e2 e2' h oev2);
+    eliminate exists e2' oev2. step e2 e2' h oev2 returns exists e' oev. step (EPair e1 e2) e' h oev with st. begin
       bind_squash st (fun st -> return_squash (PairRight e1 st))
     end;
     false_elim ()
@@ -894,82 +777,58 @@ let rec destruct_steps_epair
   (e1:closed_exp)
   (e2:closed_exp)
   (e':closed_exp)
-  (lt:local_trace [])
-  (st:steps (EPair e1 e2) e' lt) :
-  Pure (value * value)
-    (requires
-      irred e' /\ ///\
+  (h:history)
+  (lt:local_trace h)
+  (st:steps (EPair e1 e2) e' h lt) :
+  Pure (value * value * (lt1:local_trace h & (lt2:local_trace (h++lt1) & local_trace (((h++lt1)++lt2)))))
+    (requires irred e' (h++lt) /\ ///\
       safe e1 /\
       safe e2) (** CA: not sure if necessary **)
-    (ensures fun (e1', e2') ->
-      exists lt1 lt2 lt_f.
-      (steps e1 e1' lt1 /\
-       steps e2 e2' lt2 /\
-       well_formed_local_trace [] (lt1 @ lt2) /\
-       steps (EPair e1 e2) (EPair e1' e2') (lt1 @ lt2) /\
-       steps (EPair e1' e2') e' lt_f /\
-       lt == (lt1 @ lt2) @ lt_f))
+    (ensures fun (e1', e2', (| lt1, (| lt2, lt3 |) |)) ->
+      steps e1 e1' h lt1 /\
+      steps e2 e2' (h++lt1) lt2 /\
+      steps (EPair e1 e2) (EPair e1' e2') h (lt1 @ lt2) /\
+      steps (EPair e1' e2') e' ((h++lt1)++lt2) lt3  /\
+      lt == ((lt1 @ lt2) @ lt3) /\
+      (irred e1 h ==> (lt1 == [] /\ e1 == e1')) /\
+      (irred e2 (h++lt1) ==> (lt2 == [] /\ e2 == e2')))
     (decreases st)
   = match st with
-    | SRefl (EPair e1 e2) -> begin
-      srefl_epair_implies_value e1 e2;
-      (e1, e2, [], [], [])
+    | SRefl (EPair e1 e2) h -> begin
+      srefl_epair_implies_value e1 e2 h;
+      (e1, e2, (| [], (| [], [] |) |))
       end
-    | STrans #f1 #f2 #f3 #lt_f2_f3 #oev_f1_f2 step_epair step_epair_steps -> begin
-      let (EPair e1 e2) = f1 in
-      let e' = f3 in
+    | STrans #e #f2 #e' #h #_ #lt23 step_epair step_epair_steps -> begin
+      let (EPair e1 e2) = e in
       match step_epair with
-      | PairLeft #e1 e2 #e1' #oev1 step_e1 -> begin
+      | PairLeft #e1 e2 #e1' #h #oev1 step_e1 -> begin
         let (EPair e1' e2) = f2 in
-        singleton_no_history_trivially_well_formed oev1;
-        lem_step_implies_steps e1 e1' oev1;
-        lem_step_implies_steps (EPair e1 e2) (EPair e1' e2) oev_f1_f2;
-        let lt1 = if Some? oev1 then ([] @ [Some?.v oev1]) else [] in
-        assert (steps e1 e1' lt1);
-        assert (steps (EPair e1 e2) (EPair e1' e2) lt1);
-        assert (steps e2 e2 []);
-        lem_steps_preserve_safe e1 e1' lt1;
-        let s2 : steps (EPair e1' e2) e' lt_f2_f3 = step_epair_steps in
-        let (e1'', e2'', lt1'', lt2'', lt_f'') = destruct_steps_epair e1' e2 e' lt_f2_f3 s2 in
-        assume (well_formed_local_trace [] (lt1 @ lt1''));
-        lem_steps_transitive e1 e1' e1'' lt1 lt1'';
-        assume (well_formed_local_trace [] (lt1 @ (lt1'' @ lt2'')));
-        lem_steps_transitive (EPair e1 e2) (EPair e1' e2) (EPair e1'' e2'') lt1 (lt1'' @ lt2'');
-        (*assert (steps e1 e1'' (lt1 @ lt1''));
-        assert (steps e2 e2'' lt2'');
-        assume (well_formed_local_trace [] ((lt1 @ lt1'') @ lt2''));
-        assert (steps (EPair e1 e2) (EPair e1'' e2'') ((lt1 @ lt1'') @ lt2''));
-        assert (steps (EPair e1'' e2'') e' lt_f'');
-        assume (lt == ((lt1 @ lt1'') @ lt2'') @ lt_f'');*)
-        assert (steps e1 e1'' (lt1 @ lt1''));
-        admit ()
-        (*assume (steps e1 e1'' lt1'');
-        assume (steps e2 e2'' lt2'');
-        assume (well_formed_local_trace [] (lt1'' @ lt2''));
-        assume (steps (EPair e1 e2) (EPair e1'' e2'') (lt1'' @ lt2''));
-        assume (steps (EPair e1'' e2'') e' lt_f'');
-        assume (lt == (lt1'' @ lt2'') @ lt_f'');*)
-        //(e1'', e2'', lt1'', lt2'', lt_f'')
+        lem_step_implies_steps e1 e1' h oev1;
+        lem_step_implies_steps (EPair e1 e2) (EPair e1' e2) h oev1;
+        let lt1 : local_trace h = get_event_trace oev1 in
+        lem_steps_preserve_safe e1 e1' h lt1;
+        let s2 : steps (EPair e1' e2) e' (h++lt1) lt23 = step_epair_steps in
+        let (e1'', e2', (| lt1', (| lt2, lt3 |) |)) = destruct_steps_epair e1' e2 e' (h++lt1) lt23 s2 in
+        lem_steps_transitive e1 e1' e1'' h lt1 lt1';
+        lem_steps_transitive (EPair e1 e2) (EPair e1' e2) (EPair e1'' e2') h lt1 (lt1' @ lt2);
+        (e1'', e2', (| (lt1 @ lt1'), (| lt2, lt3 |) |))
         end
-      | _ -> admit ()  
-        end
-        
-     (*   (e1'', e2'')
-        end
-      | PairRight e1 #e2 #e2' step_e2 -> begin
+      | PairRight e1 #e2 #e2' #h #oev2 step_e2 -> begin
         let (EPair e1 e2') = f2 in
-        lem_step_implies_steps e2 e2';
-        lem_step_implies_steps (EPair e1 e2) (EPair e1 e2');
-        lem_steps_preserve_safe e2 e2';
-        let s2 : steps (EPair e1 e2') e' = step_epair_steps in
-        let (e1'', e2'') = destruct_steps_epair e1 e2' e' s2 in
-        lem_steps_transitive e2 e2' e2'';
-        lem_steps_transitive (EPair e1 e2) (EPair e1 e2') (EPair e1'' e2'');
-        (e1'', e2'')
+        lem_step_implies_steps e2 e2' h oev2;
+        lem_step_implies_steps (EPair e1 e2) (EPair e1 e2') h oev2;
+        let lt2 : local_trace h = get_event_trace oev2 in
+        lem_steps_preserve_safe e2 e2' h lt2;
+        let s2 : steps (EPair e1 e2') e' (h++lt2) lt23 = step_epair_steps in
+        let (e1', e2'', (| lt1, (| lt2', lt3 |) |)) = destruct_steps_epair e1 e2' e' (h++lt2) lt23 s2 in
+        lem_steps_transitive e2 e2' e2'' h lt2 lt2';
+        lem_steps_transitive (EPair e1 e2) (EPair e1 e2') (EPair e1' e2'') h lt2 lt2';
+        (e1', e2'', (| lt1, (| (lt2 @ lt2'), lt3 |) |)) 
         end
-      | _ -> (e1, e2)
-      end*)
-
+      | _ -> 
+        (e1, e2, (| [], (| [], [] |) |))
+      end
+        
   (**
     How the steps look like:
       EPair e1 e2 -->* EPair e1' e2' == e'
@@ -978,27 +837,28 @@ let rec destruct_steps_epair
 
 let lem_destruct_steps_epair
   (e1' e2':closed_exp)
-  (e':closed_exp) :
-  Lemma (requires (steps (EPair e1' e2') e' /\ irred e1' /\ irred e2'))
+  (e':closed_exp) 
+  (h:history)
+  (lt:local_trace h) :
+  Lemma (requires (steps (EPair e1' e2') e' h lt /\ irred e1' h /\ irred e2' h))
         (ensures ((EPair e1' e2') == e')) = admit ()
 
-let can_step_efst_when_safe (e12:closed_exp) (t1 t2:typ) : Lemma
+let can_step_efst_when_safe (e12:closed_exp) (t1 t2:typ) (h:history) : Lemma
   (requires
     safe e12 /\
     sem_expr_shape (TPair t1 t2) e12)
-  (ensures (exists e'. step (EFst e12) e'))
+  (ensures (exists e' oev. step (EFst e12) e' h oev))
   =
-  introduce irred e12 ==> (exists e'. step (EFst e12) e') with _.
-  begin
+  introduce irred e12 h ==> (exists e' oev. step (EFst e12) e' h oev) with _. begin
+    assert (steps e12 e12 h []);
     let (EPair e1 e2) = e12 in
-    let st : step (EFst (EPair e1 e2)) e1 = FstPairReturn in
+    let st : step (EFst (EPair e1 e2)) e1 h None = FstPairReturn h in
     ()
   end;
-  introduce ~(irred e12) ==> (exists e'. step (EFst e12) e') with _.
-  begin
-    assert (exists e12'. step e12 e12');
-    eliminate exists e12'. step e12 e12' returns exists e'. step (EFst e12) e' with st.
-    begin
+  
+  introduce ~(irred e12 h) ==> (exists e' oev. step (EFst e12) e' h oev) with _. begin
+    assert (exists e12' oev12. step e12 e12' h oev12);
+    eliminate exists e12' oev12. step e12 e12' h oev12 returns exists e' oev. step (EFst e12) e' h oev with st. begin
       bind_squash st (fun st -> return_squash (FstPair st))
     end
   end
@@ -1006,46 +866,50 @@ let can_step_efst_when_safe (e12:closed_exp) (t1 t2:typ) : Lemma
 let rec destruct_steps_epair_fst
   (e12:closed_exp)
   (e':closed_exp)
-  (st:steps (EFst e12) e')
+  (h:history)
+  (lt:local_trace h)
+  (st:steps (EFst e12) e' h lt)
   (t1:typ)
   (t2:typ) :
-  Pure value
-    (requires irred e' /\
+  Pure (value * (lt12:local_trace h & local_trace (h++lt12)))
+    (requires irred e' (h++lt) /\
       safe e12 /\
       sem_expr_shape (TPair t1 t2) e12) (** CA: not sure if necessary **)
-    (ensures fun e12' ->
-      irred e12' /\
-      steps e12 e12' /\
+    (ensures fun (e12', (| lt12, lt_f |)) ->
+      irred e12' (h++lt12) /\
+      steps e12 e12' h lt12 /\
       is_closed (EFst e12') /\
-      steps (EFst e12') e')
+      steps (EFst e12') e' (h++lt12) lt_f /\
+      lt == (lt12 @ lt_f) /\
+      (irred e12 h ==> (lt12 == [] /\ e12 == e12')))
     (decreases st)
-  =
-  match st with
-  | SRefl (EFst e12) -> begin
-    can_step_efst_when_safe e12 t1 t2;
-    false_elim ()
-    end
-  | STrans #f1 #f2 #f3 step_efst step_efst_steps -> begin
-    let (EFst e12) = f1 in
-    let e' = f3 in
-    match step_efst with
-    | FstPair #e12 #e12' step_e12 -> begin
-      let (EFst e12') = f2 in
-      lem_step_implies_steps e12 e12';
-      lem_step_implies_steps (EFst e12) (EFst e12');
-      lem_steps_preserve_safe e12 e12';
-      lem_steps_preserve_sem_expr_shape e12 e12' (TPair t1 t2);
-      let s2 : steps (EFst e12') e' = step_efst_steps in
-      let e12'' = destruct_steps_epair_fst e12' e' s2 t1 t2 in
-      lem_steps_transitive e12 e12' e12'';
-      e12''
+  = match st with
+    | SRefl (EFst e12) h -> begin
+      can_step_efst_when_safe e12 t1 t2 h;
+      false_elim ()
       end
-    | FstPairReturn #e1 #e2 -> begin
-      lem_step_implies_steps (EFst (EPair e1 e2)) e1;
-      e12
+    | STrans #e #f2 #e' #h #_ #lt23 step_efst step_efst_steps -> begin
+      let (EFst e12) = e in
+      match step_efst with
+      | FstPair #e12 #e12' #h #oev12 step_e12 -> begin
+        let (EFst e12') = f2 in
+        lem_step_implies_steps e12 e12' h oev12;
+        lem_step_implies_steps (EFst e12) (EFst e12') h oev12;
+        let lt12 : local_trace h = get_event_trace oev12 in
+        lem_steps_preserve_safe e12 e12' h lt12;
+        lem_steps_preserve_sem_expr_shape e12 e12' h lt12 (TPair t1 t2);
+        let s2 : steps (EFst e12') e' (h++lt12) lt23 = step_efst_steps in
+        let (e12'', (| lt12', lt_f |)) = destruct_steps_epair_fst e12' e' (h++lt12) lt23 s2 t1 t2 in
+        lem_steps_transitive e12 e12' e12'' h lt12 lt12';
+        (e12'', (| (lt12 @ lt12'), lt_f |))
       end
-    | _ -> false_elim ()
-    end
+      | FstPairReturn #e1 #e2 h -> begin
+        lem_step_implies_steps (EFst (EPair e1 e2)) e1 h None;
+        assert (steps e12 e12 h []);
+        (e12, (| [], lt |))
+        end
+      | _ -> false_elim ()
+      end
 
   (**
     How the steps look like:
@@ -1054,27 +918,28 @@ let rec destruct_steps_epair_fst
 
 let lem_destruct_steps_epair_fst
   (e1 e2:closed_exp)
-  (e':closed_exp) :
-  Lemma (requires (steps (EFst (EPair e1 e2)) e' /\ irred e1 /\ irred e2))
+  (e':closed_exp) 
+  (h:history) 
+  (lt:local_trace h) :
+  Lemma (requires (steps (EFst (EPair e1 e2)) e' h lt /\ irred e1 h /\ irred e2 h))
         (ensures (e1 == e')) = admit ()
 
-let can_step_esnd_when_safe (e12:closed_exp) (t1 t2:typ) : Lemma
+let can_step_esnd_when_safe (e12:closed_exp) (t1 t2:typ) (h:history) : Lemma
   (requires
     safe e12 /\
     sem_expr_shape (TPair t1 t2) e12)
-  (ensures (exists e'. step (ESnd e12) e'))
+  (ensures (exists e' oev. step (ESnd e12) e' h oev))
   =
-  introduce irred e12 ==> (exists e'. step (ESnd e12) e') with _.
-  begin
+  introduce irred e12 h ==> (exists e' oev. step (ESnd e12) e' h oev) with _. begin
+    assert (steps e12 e12 h []);
     let (EPair e1 e2) = e12 in
-    let st : step (ESnd (EPair e1 e2)) e2 = SndPairReturn in
+    let st : step (ESnd (EPair e1 e2)) e2 h None = SndPairReturn h in
     ()
   end;
-  introduce ~(irred e12) ==> (exists e'. step (ESnd e12) e') with _.
-  begin
-    assert (exists e12'. step e12 e12');
-    eliminate exists e12'. step e12 e12' returns exists e'. step (ESnd e12) e' with st.
-    begin
+  
+  introduce ~(irred e12 h) ==> (exists e' oev. step (ESnd e12) e' h oev) with _. begin
+    assert (exists e12' oev12. step e12 e12' h oev12);
+    eliminate exists e12' oev12. step e12 e12' h oev12 returns exists e' oev. step (ESnd e12) e' h oev with st. begin
       bind_squash st (fun st -> return_squash (SndPair st))
     end
   end
@@ -1082,46 +947,50 @@ let can_step_esnd_when_safe (e12:closed_exp) (t1 t2:typ) : Lemma
 let rec destruct_steps_epair_snd
   (e12:closed_exp)
   (e':closed_exp)
-  (st:steps (ESnd e12) e')
+  (h:history)
+  (lt:local_trace h)
+  (st:steps (ESnd e12) e' h lt)
   (t1:typ)
   (t2:typ) :
-  Pure value
-    (requires irred e' /\
+  Pure (value * (lt12:local_trace h & local_trace (h++lt12)))
+    (requires irred e' (h++lt) /\
       safe e12 /\
       sem_expr_shape (TPair t1 t2) e12) (** CA: not sure if necessary **)
-    (ensures fun e12' ->
-      irred e12' /\
-      steps e12 e12' /\
+    (ensures fun (e12', (| lt12, lt_f |)) ->
+      irred e12' (h++lt12) /\
+      steps e12 e12' h lt12 /\
       is_closed (ESnd e12') /\
-      steps (ESnd e12') e')
+      steps (ESnd e12') e' (h++lt12) lt_f /\
+      lt == (lt12 @ lt_f) /\
+      (irred e12 h ==> (lt12 == [] /\ e12 == e12')))
     (decreases st)
-  =
-  match st with
-  | SRefl (ESnd e12) -> begin
-    can_step_esnd_when_safe e12 t1 t2;
-    false_elim ()
-    end
-  | STrans #f1 #f2 #f3 step_esnd step_esnd_steps -> begin
-    let (ESnd e12) = f1 in
-    let e' = f3 in
-    match step_esnd with
-    | SndPair #e12 #e12' step_e12 -> begin
-      let (ESnd e12') = f2 in
-      lem_step_implies_steps e12 e12';
-      lem_step_implies_steps (ESnd e12) (ESnd e12');
-      lem_steps_preserve_safe e12 e12';
-      lem_steps_preserve_sem_expr_shape e12 e12' (TPair t1 t2);
-      let s2 : steps (ESnd e12') e' = step_esnd_steps in
-      let e12'' = destruct_steps_epair_snd e12' e' s2 t1 t2 in
-      lem_steps_transitive e12 e12' e12'';
-      e12''
+  = match st with
+    | SRefl (ESnd e12) h -> begin
+      can_step_esnd_when_safe e12 t1 t2 h;
+      false_elim ()
       end
-    | SndPairReturn #e1 #e2 -> begin
-      lem_step_implies_steps (ESnd (EPair e1 e2)) e2;
-      e12
+    | STrans #e #f2 #e' #h #_ #lt23 step_esnd step_esnd_steps -> begin
+      let (ESnd e12) = e in
+      match step_esnd with
+      | SndPair #e12 #e12' #h #oev12 step_e12 -> begin
+        let (ESnd e12') = f2 in
+        lem_step_implies_steps e12 e12' h oev12;
+        lem_step_implies_steps (ESnd e12) (ESnd e12') h oev12;
+        let lt12 : local_trace h = get_event_trace oev12 in
+        lem_steps_preserve_safe e12 e12' h lt12;
+        lem_steps_preserve_sem_expr_shape e12 e12' h lt12 (TPair t1 t2);
+        let s2 : steps (ESnd e12') e' (h++lt12) lt23 = step_esnd_steps in
+        let (e12'', (| lt12', lt_f |)) = destruct_steps_epair_snd e12' e' (h++lt12) lt23 s2 t1 t2 in
+        lem_steps_transitive e12 e12' e12'' h lt12 lt12';
+        (e12'', (| (lt12 @ lt12'), lt_f |))
+        end
+      | SndPairReturn #e1 #e2 h -> begin
+        lem_step_implies_steps (ESnd (EPair e1 e2)) e2 h None;
+        assert (steps e12 e12 h []);
+        (e12, (| [], lt |))
+        end
+      | _ -> false_elim ()
       end
-    | _ -> false_elim ()
-    end
 
   (**
     How the steps look like:
@@ -1130,6 +999,8 @@ let rec destruct_steps_epair_snd
 
 let lem_destruct_steps_epair_snd
   (e1 e2:closed_exp)
-  (e':closed_exp) :
-  Lemma (requires (steps (ESnd (EPair e1 e2)) e' /\ irred e1 /\ irred e2))
+  (e':closed_exp) 
+  (h:history) 
+  (lt:local_trace h) :
+  Lemma (requires (steps (ESnd (EPair e1 e2)) e' h lt /\ irred e1 h /\ irred e2 h))
         (ensures (e2 == e')) = admit ()
